\documentclass[10pt,landscape]{article}
\usepackage[top=15truemm,bottom=15truemm,left=15truemm,right=15truemm]{geometry}
\usepackage{bussproofs}
\usepackage{ascmac,amsmath,amssymb,amsbsy}
\usepackage{graphics}

\newcommand{\mini}[1]{\scalebox{0.7}{#1}}

\begin{document}

\section*{Syntax}

\vspace{30pt}

\begin{alignat*}{2}
    \boldsymbol{i} & \in \mathbf{Int} & &\\
    \boldsymbol{b} & \in \mathbf{Bool} & &\\
    \boldsymbol{x,y} & \in \mathbf{Var} & &\\
    \boldsymbol{op} & \in \mathbf{Prim} & ~ ::= & ~~ \boldsymbol{+} \mid \boldsymbol{-} \mid \boldsymbol{*} \mid \boldsymbol{<}\\
    \boldsymbol{v} & \in \mathbf{Value} & ~ ::= & ~~ \boldsymbol{i} \mid \boldsymbol{b} \mid (\boldsymbol{\mathcal{E}})[\mathtt{fun} ~ \boldsymbol{x} \to \boldsymbol{e}] \mid (\boldsymbol{\mathcal{E}})[\mathtt{rec} ~ \boldsymbol{x} = \mathtt{fun} ~ \boldsymbol{y} \to \boldsymbol{e}] \mid \boldsymbol{[]} \mid \boldsymbol{v} :: \boldsymbol{v}\\
    \boldsymbol{\mathcal{E}} & \in \mathbf{Env} & ~ ::= & ~~ \bullet \mid \boldsymbol{\mathcal{E}},\boldsymbol{x} = \boldsymbol{v}\\
    \boldsymbol{e} & \in \mathbf{Exp} & ~ ::= & ~~ \boldsymbol{i}
    \mid \boldsymbol{b}
    \mid \boldsymbol{x}
    \mid \boldsymbol{e ~ op ~ e}
    \mid \mathtt{if} ~ \boldsymbol{e} ~ \mathtt{then} ~ \boldsymbol{e} ~ \mathtt{else} ~ \boldsymbol{e}
    \mid \mathtt{let} ~ \boldsymbol{x = e} ~ \mathtt{in} ~ \boldsymbol{e}\\
    &&&\mid \mathtt{fun} ~ \boldsymbol{x} \to \boldsymbol{e}
    \mid \boldsymbol{e ~ e}
    \mid \mathtt{let ~ rec} ~ \boldsymbol{x} = \mathtt{fun} ~ \boldsymbol{y} \to \boldsymbol{e} ~ \mathtt{in} ~ \boldsymbol{e}\\
    &&&\mid \boldsymbol{[]}
    \mid \boldsymbol{e} :: \boldsymbol{e}
    \mid \mathtt{match} ~ \boldsymbol{e} ~ \mathtt{with} ~ \boldsymbol{[]} \to \boldsymbol{e} ~ \boldsymbol{|} ~ \boldsymbol{x} :: \boldsymbol{y} \to \boldsymbol{e}
\end{alignat*}

\newpage

\section*{Derivation Rules}

\vspace{30pt}

\begin{center}
    \AxiomC{${}_{}$}
    \RightLabel{(E-I\mini{NT})}
    \UnaryInfC{$\boldsymbol{\mathcal{E}} \vdash \boldsymbol{i} \Downarrow \boldsymbol{i}$}
    \DisplayProof
    \hspace{12pt}
    \AxiomC{${}_{}$}
    \RightLabel{(E-B\mini{OOL})}
    \UnaryInfC{$\boldsymbol{\mathcal{E}} \vdash \boldsymbol{b} \Downarrow \boldsymbol{b}$}
    \DisplayProof
    \hspace{12pt}
    \AxiomC{$(\boldsymbol{\mathcal{E}}(\boldsymbol{x}) = \boldsymbol{v})$}
    \RightLabel{(E-V\mini{AR})}
    \UnaryInfC{$\boldsymbol{\mathcal{E}} \vdash \boldsymbol{x} \Downarrow \boldsymbol{v}$}
    \DisplayProof
\end{center}

\vspace{-5pt}

\begin{center}
    \AxiomC{$\boldsymbol{\mathcal{E}} \vdash \boldsymbol{e_1} \Downarrow \boldsymbol{i_1}$}
    \AxiomC{$\boldsymbol{\mathcal{E}} \vdash \boldsymbol{e_2} \Downarrow \boldsymbol{i_2}$}
    \AxiomC{$\boldsymbol{i_1} ~ \mathtt{plus} ~ \boldsymbol{i_2} ~ \mathtt{is} ~ \boldsymbol{i_3}$}
    \RightLabel{(E-P\mini{LUS})}
    \TrinaryInfC{$\boldsymbol{\mathcal{E}} \vdash \boldsymbol{e_1 + e_2} \Downarrow \boldsymbol{i_3}$}
    \DisplayProof
    \hspace{12pt}
    \AxiomC{$\boldsymbol{\mathcal{E}} \vdash \boldsymbol{e_1} \Downarrow \boldsymbol{i_1}$}
    \AxiomC{$\boldsymbol{\mathcal{E}} \vdash \boldsymbol{e_2} \Downarrow \boldsymbol{i_2}$}
    \AxiomC{$\boldsymbol{i_1} ~ \mathtt{minus} ~ \boldsymbol{i_2} ~ \mathtt{is} ~ \boldsymbol{i_3}$}
    \RightLabel{(E-M\mini{INUS})}
    \TrinaryInfC{$\boldsymbol{\mathcal{E}} \vdash \boldsymbol{e_1 - e_2} \Downarrow \boldsymbol{i_3}$}
    \DisplayProof
\end{center}

\vspace{-5pt}

\begin{center}
    \AxiomC{$\boldsymbol{\mathcal{E}} \vdash \boldsymbol{e_1} \Downarrow \boldsymbol{i_1}$}
    \AxiomC{$\boldsymbol{\mathcal{E}} \vdash \boldsymbol{e_2} \Downarrow \boldsymbol{i_2}$}
    \AxiomC{$\boldsymbol{i_1} ~ \mathtt{times} ~ \boldsymbol{i_2} ~ \mathtt{is} ~ \boldsymbol{i_3}$}
    \RightLabel{(E-T\mini{IMES})}
    \TrinaryInfC{$\boldsymbol{\mathcal{E}} \vdash \boldsymbol{e_1 * e_2} \Downarrow \boldsymbol{i_3}$}
    \DisplayProof
    \hspace{12pt}
    \AxiomC{$\boldsymbol{\mathcal{E}} \vdash \boldsymbol{e_1} \Downarrow \boldsymbol{i_1}$}
    \AxiomC{$\boldsymbol{\mathcal{E}} \vdash \boldsymbol{e_2} \Downarrow \boldsymbol{i_2}$}
    \AxiomC{$\boldsymbol{i_1} ~ \mathtt{less ~ than} ~ \boldsymbol{i_2} ~ \mathtt{is} ~ \boldsymbol{b_3}$}
    \RightLabel{(E-L\mini{T})}
    \TrinaryInfC{$\boldsymbol{\mathcal{E}} \vdash \boldsymbol{e_1 < e_2} \Downarrow \boldsymbol{b_3}$}
    \DisplayProof
\end{center}

\vspace{-5pt}

\begin{center}
    \AxiomC{$\boldsymbol{\mathcal{E}} \vdash \boldsymbol{e_1} \Downarrow \mathtt{true}$}
    \AxiomC{$\boldsymbol{\mathcal{E}} \vdash \boldsymbol{e_2} \Downarrow \boldsymbol{v}$}
    \RightLabel{(E-I\mini{F}T)}
    \BinaryInfC{$\boldsymbol{\mathcal{E}} \vdash \mathtt{if} ~ \boldsymbol{e_1} ~ \mathtt{then} ~ \boldsymbol{e_2} ~ \mathtt{else} ~ \boldsymbol{e_3} \Downarrow \boldsymbol{v}$}
    \DisplayProof
    \hspace{12pt}
    \AxiomC{$\boldsymbol{\mathcal{E}} \vdash \boldsymbol{e_1} \Downarrow \mathtt{false}$}
    \AxiomC{$\boldsymbol{\mathcal{E}} \vdash \boldsymbol{e_3} \Downarrow \boldsymbol{v}$}
    \RightLabel{(E-I\mini{F}F)}
    \BinaryInfC{$\boldsymbol{\mathcal{E}} \vdash \mathtt{if} ~ \boldsymbol{e_1} ~ \mathtt{then} ~ \boldsymbol{e_2} ~ \mathtt{else} ~ \boldsymbol{e_3} \Downarrow \boldsymbol{v}$}
    \DisplayProof
\end{center}

\vspace{-5pt}

\begin{prooftree}
    \AxiomC{$\boldsymbol{\mathcal{E}} \vdash \boldsymbol{e_1} \Downarrow \boldsymbol{v_1}$}
    \AxiomC{$\boldsymbol{\mathcal{E}}, \boldsymbol{x} = \boldsymbol{v_1} \vdash \boldsymbol{e_2} \Downarrow \boldsymbol{v}$}
    \RightLabel{(E-L\mini{ET})}
    \BinaryInfC{$\boldsymbol{\mathcal{E}} \vdash \mathtt{let} ~ \boldsymbol{x = e_1} ~ \mathtt{in} ~ \boldsymbol{e_2} \Downarrow \boldsymbol{v}$}
\end{prooftree}

\vspace{-5pt}

\begin{prooftree}
    \AxiomC{}
    \RightLabel{(E-F\mini{UN})}
    \UnaryInfC{$\boldsymbol{\mathcal{E}} \vdash \mathtt{fun} ~ \boldsymbol{x} \to \boldsymbol{e} \Downarrow (\boldsymbol{\mathcal{E}})[\mathtt{fun} ~ \boldsymbol{x} \to \boldsymbol{e}]$}
\end{prooftree}

\vspace{-5pt}

\begin{prooftree}
    \AxiomC{$\boldsymbol{\mathcal{E}} \vdash \boldsymbol{e_1} \Downarrow (\boldsymbol{\mathcal{E}_2})[\mathtt{fun} ~ \boldsymbol{x} \to \boldsymbol{e_0}]$}
    \AxiomC{$\boldsymbol{\mathcal{E}} \vdash \boldsymbol{e_2} \Downarrow \boldsymbol{v_2}$}
    \AxiomC{$\boldsymbol{\mathcal{E}_2}, \boldsymbol{x} = \boldsymbol{v_2} \vdash \boldsymbol{e_0} \Downarrow \boldsymbol{v}$}
    \RightLabel{(E-A\mini{PP})}
    \TrinaryInfC{$\boldsymbol{\mathcal{E}} \vdash \boldsymbol{e_1 ~ e_2} \Downarrow \boldsymbol{v}$}
\end{prooftree}

\vspace{-5pt}

\begin{prooftree}
    \AxiomC{$\boldsymbol{\mathcal{E}}, \boldsymbol{x} = (\boldsymbol{\mathcal{E}})[\mathtt{rec} ~ \boldsymbol{x} = \mathtt{fun} ~ \boldsymbol{y} \to \boldsymbol{e_1}] \vdash \boldsymbol{e_2} \Downarrow \boldsymbol{v}$}
    \RightLabel{(E-L\mini{ET}R\mini{EC})}
    \UnaryInfC{$\boldsymbol{\mathcal{E}} \vdash \mathtt{let ~ rec} ~ \boldsymbol{x} = \mathtt{fun} ~ \boldsymbol{y} \to \boldsymbol{e_1} ~ \mathtt{in} ~ \boldsymbol{e_2} \Downarrow \boldsymbol{v}$}
\end{prooftree}

\vspace{-5pt}

\begin{prooftree}
    \AxiomC{$\boldsymbol{\mathcal{E}} \vdash \boldsymbol{e_1} \Downarrow (\boldsymbol{\mathcal{E}_2})[\mathtt{rec} ~ \boldsymbol{x} = \mathtt{fun} ~ \boldsymbol{y} \to \boldsymbol{e_0}]$}
    \AxiomC{$\boldsymbol{\mathcal{E}} \vdash \boldsymbol{e_2} \Downarrow \boldsymbol{v_2}$}
    \AxiomC{$\boldsymbol{\mathcal{E}_2}, \boldsymbol{x} = (\boldsymbol{\mathcal{E}_2})[\mathtt{rec} ~ \boldsymbol{x} = \mathtt{fun} ~ \boldsymbol{y} \to \boldsymbol{e_0}], \boldsymbol{y} = \boldsymbol{v_2} \vdash \boldsymbol{e_0} \Downarrow \boldsymbol{v}$}
    \RightLabel{(E-A\mini{PP}R\mini{EC})}
    \TrinaryInfC{$\boldsymbol{\mathcal{E}} \vdash \boldsymbol{e_1 ~ e_2} \Downarrow \boldsymbol{v}$}
\end{prooftree}

\vspace{-5pt}

\begin{center}
    \AxiomC{${}$}
    \RightLabel{(E-N\mini{IL})}
    \UnaryInfC{$\boldsymbol{\mathcal{E}} \vdash \boldsymbol{[]} \Downarrow \boldsymbol{[]}$}
    \DisplayProof
    \hspace{12pt}
    \AxiomC{$\boldsymbol{\mathcal{E}} \vdash \boldsymbol{e_1} \Downarrow \boldsymbol{v_1}$}
    \AxiomC{$\boldsymbol{\mathcal{E}} \vdash \boldsymbol{e_2} \Downarrow \boldsymbol{v_2}$}
    \RightLabel{(E-C\mini{ONS})}
    \BinaryInfC{$\boldsymbol{\mathcal{E}} \vdash \boldsymbol{e_1} :: \boldsymbol{e_2} \Downarrow \boldsymbol{v_1} :: \boldsymbol{v_2}$}
    \DisplayProof
\end{center}

\vspace{-5pt}

\begin{center}
    \AxiomC{$\boldsymbol{\mathcal{E}} \vdash \boldsymbol{e_1} \Downarrow \boldsymbol{[]}$}
    \AxiomC{$\boldsymbol{\mathcal{E}} \vdash \boldsymbol{e_2} \Downarrow \boldsymbol{v}$}
    \RightLabel{(E-M\mini{ATCH}N\mini{IL})}
    \BinaryInfC{$\boldsymbol{\mathcal{E}} \vdash \mathtt{match} ~ \boldsymbol{e_1} ~ \mathtt{with} ~ \boldsymbol{[]} \to \boldsymbol{e_2} ~ \boldsymbol{|} ~ \boldsymbol{x} :: \boldsymbol{y} \to \boldsymbol{e_3} \Downarrow \boldsymbol{v}$}
    \DisplayProof
    \hspace{12pt}
    \AxiomC{$\boldsymbol{\mathcal{E}} \vdash \boldsymbol{e_1} \Downarrow \boldsymbol{v_1} :: \boldsymbol{v_2}$}
    \AxiomC{$\boldsymbol{\mathcal{E}}, \boldsymbol{x} = \boldsymbol{v_1}, \boldsymbol{y} = \boldsymbol{v_2} \vdash \boldsymbol{e_3} \Downarrow \boldsymbol{v}$}
    \RightLabel{(E-M\mini{ATCH}C\mini{ONS})}
    \BinaryInfC{$\boldsymbol{\mathcal{E}} \vdash \mathtt{match} ~ \boldsymbol{e_1} ~ \mathtt{with} ~ \boldsymbol{[]} \to \boldsymbol{e_2} ~ \boldsymbol{|} ~ \boldsymbol{x} :: \boldsymbol{y} \to \boldsymbol{e_3} \Downarrow \boldsymbol{v}$}
    \DisplayProof
\end{center}

\vspace{-5pt}

\begin{center}
    \AxiomC{$(\boldsymbol{i_3} = \boldsymbol{i_1 + i_2})$}
    \RightLabel{(B-P\mini{LUS})}
    \UnaryInfC{$\boldsymbol{i_1} ~ \mathtt{plus} ~ \boldsymbol{i_2} ~ \mathtt{is} ~ \boldsymbol{i_3}$}
    \DisplayProof
    \hspace{12pt}
    \AxiomC{$(\boldsymbol{i_3} = \boldsymbol{i_1 - i_2})$}
    \RightLabel{(B-M\mini{INUS})}
    \UnaryInfC{$\boldsymbol{i_1} ~ \mathtt{minus} ~ \boldsymbol{i_2} ~ \mathtt{is} ~ \boldsymbol{i_3}$}
    \DisplayProof
    \hspace{12pt}
    \AxiomC{$(\boldsymbol{i_3} = \boldsymbol{i_1 * i_2})$}
    \RightLabel{(B-T\mini{IMES})}
    \UnaryInfC{$\boldsymbol{i_1} ~ \mathtt{times} ~ \boldsymbol{i_2} ~ \mathtt{is} ~ \boldsymbol{i_3}$}
    \DisplayProof
    \hspace{12pt}
    \AxiomC{$(\boldsymbol{b_3} = (\boldsymbol{i_1 < i_2}))$}
    \RightLabel{(B-L\mini{T})}
    \UnaryInfC{$\boldsymbol{i_1} ~ \mathtt{less ~ than} ~ \boldsymbol{i_2} ~ \mathtt{is} ~ \boldsymbol{b_3}$}
    \DisplayProof
\end{center}

\end{document}

